Work on evaluate_skip proof

compiler/repl/evaluate_skipScript.sml
@@ -5,6 +5,7 @@
 *)
 open preamble
 open evaluateTheory semanticPrimitivesTheory evaluatePropsTheory
+local open helperLib ml_progTheory in end
 
 val _ = new_theory "evaluate_skip";
 
@@ -47,6 +48,10 @@ Inductive v_rel:
   (∀fr ft fe env1 env2 fns n.
      v_rel fr ft fe (Recclosure env1 fns n) (Recclosure env2 fns n))
   ∧
+  (∀fr ft fe env1 env2 ns.
+    env_rel fr ft fe env1 env2 ⇒
+     v_rel fr ft fe (Env env1 ns) (Env env2 ns))
+  ∧
   (∀fr ft fe env1 env2.
      ctor_rel ft fe env1.c env2.c ∧
      (∀n. nsLookup env1.v n = NONE ⇒ nsLookup env2.v n = NONE) ∧
@@ -54,6 +59,24 @@ Inductive v_rel:
             ∃w. nsLookup env2.v n = SOME w ∧ v_rel fr ft fe v w) ⇒
      env_rel fr ft fe env1 env2)
 End
+
+Theorem v_rel_def =
+  [“v_rel fr ft fe (Conv opt vs) v”,
+   “v_rel fr ft fe (Closure env n x) v”,
+   “v_rel fr ft fe (Recclosure env f n) v”,
+   “v_rel fr ft fe (Vectorv vs) v”,
+   “v_rel fr ft fe (Litv lit) v”,
+   “v_rel fr ft fe (Loc loc) v”,
+   “v_rel fr ft fe (Env env ns) v”,
+   “v_rel fr ft fe v (Conv opt vs)”,
+   “v_rel fr ft fe v (Closure env n x)”,
+   “v_rel fr ft fe v (Recclosure env f n)”,
+   “v_rel fr ft fe v (Vectorv vs)”,
+   “v_rel fr ft fe v (Litv lit)”,
+   “v_rel fr ft fe v (Loc loc)”,
+   “v_rel fr ft fe v (Env env ns)”]
+  |> map (SIMP_CONV (srw_ss()) [Once v_rel_cases])
+  |> LIST_CONJ;
 
 Theorem env_rel_def =
   “env_rel fr ft fe env1 env2” |> SIMP_CONV std_ss [Once v_rel_cases];
@@ -97,6 +120,14 @@ Definition res_rel_def[simp]:
   (res_rel f g (Rerr (Rabort e)) (Rerr (Rabort e1)) ⇔ e = e1) ∧
   (res_rel f g x y                                  ⇔ F)
 End
+
+Theorem res_rel_abort[simp]:
+  res_rel R Q (Rerr (Rabort x)) r ⇔ r = Rerr (Rabort x)
+Proof
+  Cases_on ‘r’ \\ gs []
+  \\ Cases_on ‘e’ \\ gs []
+  \\ rw [EQ_SYM_EQ]
+QED
 
 Theorem stamp_rel_update:
   ∀ft fe x y.
@@ -219,6 +250,1068 @@ Proof
   \\ cheat (* ref_rel_mono *)
 QED
 
+(* --------------------------------------------------------------------------
+ *
+ * -------------------------------------------------------------------------- *)
+
+Theorem pmatch_v_ok:
+  (∀envC s p v ws env.
+    pmatch envC s p v ws = Match env ⇒
+      ∀envC' s' v' ws' env'.
+        ctor_rel ft fe envC envC' ∧
+        LIST_REL (ref_rel (v_rel fr ft fe)) s s' ∧
+        v_rel fr ft fe v v' ∧
+        LIST_REL (v_rel fr ft fe) (MAP SND ws) (MAP SND ws') ∧
+        pmatch envC' s' p v' ws' = Match env' ∧
+        (∀n. if n < LENGTH s then
+             ∃m. FLOOKUP fr n = SOME m ∧ m < LENGTH s' ∧
+                 ref_rel (v_rel fr ft fe) (EL n s) (EL m s')
+           else FLOOKUP fr n = NONE) ⇒
+          LIST_REL (v_rel fr ft fe) (MAP SND env) (MAP SND env')) ∧
+  (∀envC s ps vs ws env.
+    pmatch_list envC s ps vs ws = Match env ⇒
+      ∀envC' s' vs' ws' env'.
+        ctor_rel ft fe envC envC' ∧
+        LIST_REL (ref_rel (v_rel fr ft fe)) s s' ∧
+        LIST_REL (v_rel fr ft fe) vs vs' ∧
+        LIST_REL (v_rel fr ft fe) (MAP SND ws) (MAP SND ws') ∧
+        pmatch_list envC' s' ps vs' ws' = Match env' ∧
+        (∀n. if n < LENGTH s then
+             ∃m. FLOOKUP fr n = SOME m ∧ m < LENGTH s' ∧
+                 ref_rel (v_rel fr ft fe) (EL n s) (EL m s')
+           else FLOOKUP fr n = NONE) ⇒
+          LIST_REL (v_rel fr ft fe) (MAP SND env) (MAP SND env'))
+Proof
+  ho_match_mp_tac pmatch_ind \\ rw [] \\ gvs [pmatch_def, SF SFY_ss]
+  >- (
+    gvs [CaseEq "bool", Once v_rel_cases, pmatch_def])
+  >- (
+    gvs [CaseEqs ["bool", "option", "prod"], Once v_rel_cases, pmatch_def]
+    \\ rename1 ‘pmatch _ _ _ (Conv tt _)’
+    \\ Cases_on ‘tt’ \\ gvs [pmatch_def, CaseEqs ["prod", "option", "bool"]]
+    \\ first_x_assum irule
+    \\ first_assum (irule_at Any) \\ gs [])
+  >- (
+    gvs [CaseEq "bool", Once v_rel_cases, pmatch_def]
+    \\ rename1 ‘pmatch _ _ _ (Conv tt _)’
+    \\ Cases_on ‘tt’ \\ gvs [pmatch_def, CaseEq "bool"]
+    \\ first_x_assum irule
+    \\ first_assum (irule_at Any) \\ gs [])
+  >- (
+    cheat (*
+    gvs [CaseEqs ["bool", "option", "store_v"]]
+    \\ rgs [Once v_rel_cases] \\ gvs [pmatch_def, CaseEqs ["store_v", "option"]]
+    \\ first_x_assum irule
+    \\ first_assum (irule_at Any) \\ gs []
+    \\ gvs [store_lookup_def, EVERY_EL, EL_MAP, LIST_REL_EL_EQN]
+    \\ first_x_assum (qspec_then ‘l2’ assume_tac) \\ gs [] *))
+  \\ cheat
+QED
+
+local
+  val ind_thm =
+    full_evaluate_ind
+    |> Q.SPECL [
+      ‘λs env xs. ∀res s1 l fr ft fe t env1.
+        evaluate s env xs = (s1, res) ∧
+        state_rel l fr ft fe s t ∧
+        env_rel fr ft fe env env1 ⇒
+          ∃fr1 ft1 fe1 t1 res1.
+            fr ⊑ fr1 ∧ ft ⊑ ft1 ∧ fe ⊑ fe1 ∧
+            state_rel l fr1 ft1 fe1 s1 t1 ∧
+            evaluate t env1 xs = (t1, res1) ∧
+            res_rel (LIST_REL (v_rel fr1 ft1 fe1))
+                    (v_rel fr1 ft1 fe1) res res1’,
+      ‘λs env v ps errv. ∀res s1 l fr ft fe t env1 w errw.
+        evaluate_match s env v ps errv = (s1, res) ∧
+        state_rel l fr ft fe s t ∧
+        env_rel fr ft fe env env1 ∧
+        v_rel fr ft fe v w ∧
+        v_rel fr ft fe errv errw ⇒
+          ∃fr1 ft1 fe1 t1 res1.
+            fr ⊑ fr1 ∧ ft ⊑ ft1 ∧ fe ⊑ fe1 ∧
+            state_rel l fr1 ft1 fe1 s1 t1 ∧
+            evaluate_match t env1 w ps errw = (t1, res1) ∧
+            res_rel (LIST_REL (v_rel fr1 ft1 fe1))
+                    (v_rel fr1 ft1 fe1) res res1’,
+      ‘λs env ds. ∀res s1 l fr ft fe t env1.
+        evaluate_decs s env ds = (s1, res) ∧
+        state_rel l fr ft fe s t ∧
+        env_rel fr ft fe env env1 ⇒
+          ∃fr1 ft1 fe1 t1 res1.
+            fr ⊑ fr1 ∧ ft ⊑ ft1 ∧ fe ⊑ fe1 ∧
+            state_rel l fr1 ft1 fe1 s1 t1 ∧
+            evaluate_decs t env1 ds = (t1, res1) ∧
+            res_rel (λenv' env1'.
+                       env_rel fr1 ft1 fe1 (extend_dec_env env' env)
+                                           (extend_dec_env env1' env1))
+                    (v_rel fr1 ft1 fe1) res res1’]
+    |> CONV_RULE (DEPTH_CONV BETA_CONV);
+  val ind_goals =
+    ind_thm |> concl |> dest_imp |> fst
+            |> helperLib.list_dest dest_conj
+in
+  fun get_goal s =
+    first (can (find_term (can (match_term (Term [QUOTE s]))))) ind_goals
+    |> helperLib.list_dest dest_forall
+    |> last
+  fun evaluate_update () = ind_thm |> concl |> rand
+  fun the_ind_thm () = ind_thm
+end
+
+Theorem evaluate_update_Nil:
+  ^(get_goal "[]")
+Proof
+  rw [evaluate_def]
+  \\ first_assum (irule_at Any) \\ gs []
+QED
+
+Theorem evaluate_update_Cons:
+  ^(get_goal "_::_::_")
+Proof
+  rw [evaluate_def]
+  \\ gvs [CaseEqs ["result", "prod"], PULL_EXISTS]
+  >~ [‘evaluate _ _ [_] = (_, Rerr err)’] >- (
+    first_x_assum (drule_all_then strip_assume_tac)
+    \\ Cases_on ‘res1’ \\ gs []
+    \\ rename1 ‘_ _ (Rerr err) (Rerr err1)’
+    \\ Cases_on ‘err’ \\ Cases_on ‘err1’ \\ gs []
+    \\ first_assum (irule_at Any) \\ gs []
+    \\ first_assum (irule_at Any) \\ gs [])
+  \\ first_x_assum (drule_all_then strip_assume_tac)
+  \\ Cases_on ‘res1’ \\ gs []
+  \\ drule_all_then assume_tac env_rel_update
+  \\ first_x_assum (drule_all_then strip_assume_tac)
+  \\ Cases_on ‘res1’ \\ gs []
+  \\ first_assum (irule_at Any) \\ gs []
+  \\ gs [SUBMAP_TRANS, SF SFY_ss]
+  \\ drule_then strip_assume_tac evaluate_sing \\ gvs []
+  \\ irule (CONJUNCT1 v_rel_update)
+  \\ gs [SUBMAP_TRANS, SF SFY_ss]
+  \\ first_assum (irule_at (Pos last))
+QED
+
+Theorem evaluate_update_Lit:
+  ^(get_goal "Lit l")
+Proof
+  rw [evaluate_def] \\ gs []
+  \\ first_assum (irule_at Any)
+  \\ simp [v_rel_rules]
+QED
+
+Theorem evaluate_update_Raise:
+  ^(get_goal "Raise e")
+Proof
+  rw [evaluate_def] \\ gs []
+  \\ gvs [CaseEqs ["result", "prod"], PULL_EXISTS]
+  \\ first_x_assum (drule_all_then strip_assume_tac)
+  \\ Cases_on ‘res1’ \\ gs []
+  \\ first_assum (irule_at Any) \\ gs []
+  \\ drule_then strip_assume_tac evaluate_sing \\ gvs []
+QED
+
+Theorem evaluate_update_Handle:
+  ^(get_goal "Handle e")
+Proof
+  rw [evaluate_def]
+  \\ gvs [CaseEqs ["prod", "result", "error_result"], PULL_EXISTS]
+  \\ cheat
+QED
+
+Theorem do_con_check_update:
+  env_rel fr ft fe env env1 ⇒
+  do_con_check env.c cn n = do_con_check env1.c cn n
+Proof
+  strip_tac \\ eq_tac \\ gs [env_rel_def, ctor_rel_def]
+  \\ rw [do_con_check_def]
+  \\ CASE_TAC \\ gs []
+  \\ rename1 ‘nsLookup env.c k’
+  \\ rpt (first_x_assum (qspec_then ‘k’ assume_tac)) \\ gs []
+  \\ gs [OPTREL_def]
+  \\ PairCases_on ‘x0’ \\ PairCases_on ‘y0’ \\ gs []
+QED
+
+Theorem evaluate_update_Con:
+  ^(get_goal "Con cn es")
+Proof
+  rw [evaluate_def]
+  \\ gvs [CaseEqs ["prod", "result", "option"], PULL_EXISTS]
+  \\ drule_then assume_tac do_con_check_update \\ gs []
+  >~ [‘¬do_con_check _ _ _’] >- (
+    first_assum (irule_at Any) \\ gs [])
+  \\ first_x_assum (drule_all_then strip_assume_tac)
+  \\ Cases_on ‘res1’ \\ gs []
+  \\ gs [env_rel_def, ctor_rel_def, build_conv_def]
+  \\ gvs [CaseEqs ["prod", "option"]]
+  \\ first_assum (irule_at Any) \\ gs [v_rel_rules]
+  \\ rename1 ‘nsLookup env1.c k’
+  \\ rpt (first_x_assum (qspec_then ‘k’ assume_tac))
+  \\ gs [OPTREL_def]
+  \\ PairCases_on ‘y0’ \\ gs []
+  \\ simp [v_rel_def]
+  \\ irule stamp_rel_update
+  \\ gs [SF SFY_ss]
+QED
+
+Theorem evaluate_update_Var:
+  ^(get_goal "ast$Var n")
+Proof
+  rw [evaluate_def]
+  \\ gvs [CaseEqs ["option"]]
+  \\ first_assum (irule_at Any) \\ gs [] \\ dsimp []
+  \\ gs [env_rel_def]
+QED
+
+Theorem evaluate_update_Fun:
+  ^(get_goal "ast$Fun n e")
+Proof
+  rw [evaluate_def]
+  \\ gvs [CaseEqs ["option"]]
+  \\ first_assum (irule_at Any) \\ gs []
+  \\ simp [v_rel_def]
+QED
+
+Theorem evaluate_update_Eval:
+  op = Eval ⇒ ^(get_goal "App")
+Proof
+  rw [evaluate_def]
+  \\ gvs [AllCaseEqs(), evaluateTheory.do_eval_res_def]
+  \\ first_x_assum (drule_all_then strip_assume_tac) \\ gs []
+  \\ first_assum (irule_at Any)
+  \\ Cases_on ‘res1’ \\ gs []
+  \\ dsimp []
+  \\ gs [state_rel_def, do_eval_def]
+QED
+
+Theorem do_app_update:
+  do_app (s.refs,s.ffi) op vs = res ∧
+  state_rel l fr ft fe s t ∧
+  LIST_REL (v_rel fr ft fe) vs ws ∧
+  op ≠ Opapp ∧
+  op ≠ Eval ⇒
+    ∃fr1 ft1 fe1 res1.
+      do_app (t.refs,t.ffi) op ws = res1 ∧
+      fr ⊑ fr1 ∧
+      ft ⊑ ft1 ∧
+      fe ⊑ fe1 ∧
+      OPTREL (λ((refs1,ffi1),res) ((refs1',ffi1'),res1).
+                ∃s1 t1.
+                  s1.refs = refs1 ∧ s1.ffi = ffi1 ∧
+                  t1.refs = refs1' ∧ t1.ffi = ffi1' ∧
+                  state_rel l fr1 ft1 fe1 s1 t1 ∧
+                  res_rel (v_rel fr1 ft1 fe1) (v_rel fr1 ft1 fe1) res res1)
+              res res1
+Proof
+  cheat (*
+  strip_tac
+  \\ qpat_x_assum ‘do_app _ _ _ = _’ mp_tac
+  \\ Cases_on ‘op = Env_id’ \\ gs []
+  >- (
+    rw [semanticPrimitivesPropsTheory.do_app_cases] \\ gs []
+    \\ simp [Once v_rel_cases]
+    v_rel
+    gs [SF SFY_ss]
+    \\ simp [v_ok_def, nat_to_v_def]
+    \\ first_assum (irule_at Any) \\ gs [SF SFY_ss]
+    )
+  \\ Cases_on ‘∃chn. op = FFI chn’ \\ gs []
+  >- (
+    rw [do_app_cases] \\ gs []
+    \\ gvs [ffiTheory.call_FFI_def, store_lookup_def, store_assign_def,
+            CaseEqs ["bool", "list", "option", "oracle_result",
+                     "ffi$ffi_result"], EVERY_EL, EL_LUPDATE]
+    \\ rw [v_ok_def, EL_APPEND_EQN]
+    \\ first_assum (irule_at Any)
+    \\ csimp [oEL_LUPDATE]
+    \\ rw [] \\ gs [NOT_LESS, LESS_OR_EQ, ok_event_def, ref_ok_def, SF SFY_ss]
+    \\ irule kernel_loc_ok_LUPDATE1 \\ gs []
+    \\ strip_tac \\ gvs [v_ok_def])
+  \\ Cases_on ‘op = ConfigGC’ \\ gs []
+  >- (
+    rw [do_app_cases, oEL_LUPDATE] \\ gs [SF SFY_ss]
+    \\ simp [v_ok_def]
+    \\ first_assum (irule_at Any) \\ gs [])
+  \\ Cases_on ‘op = ListAppend’ \\ gs []
+  >- (
+    rw [do_app_cases] \\ gs []
+    \\ dxrule_all_then assume_tac v_ok_v_to_list
+    \\ dxrule_all_then assume_tac v_ok_v_to_list
+    \\ ‘EVERY (v_ok ctxt) (xs ++ ys)’
+      by gs []
+    \\ pop_assum mp_tac
+    \\ rename1 ‘EVERY (v_ok ctxt) zs ⇒ _’
+    \\ qid_spec_tac ‘zs’
+    \\ Induct \\ simp [list_to_v_def, v_ok_def]
+    \\ rw [] \\ first_assum (irule_at Any) \\ gs [SF SFY_ss])
+  \\ Cases_on ‘op = Aw8sub_unsafe’ \\ gs []
+  >- (
+    rw [do_app_cases] \\ gs []
+    \\ simp [v_ok_def]
+    \\ first_assum (irule_at Any) \\ gs [SF SFY_ss])
+  \\ Cases_on ‘op = Aw8update_unsafe’ \\ gs []
+  >- (
+    rw [do_app_cases] \\ gs [v_ok_def]
+    \\ gvs [store_lookup_def, store_assign_def, EVERY_EL, EL_LUPDATE]
+    \\ first_assum (irule_at Any) \\ gs []
+    \\ rw [SF CONJ_ss, oEL_LUPDATE] \\ gs [ref_ok_def, SF SFY_ss]
+    \\ irule kernel_loc_ok_LUPDATE1 \\ gs []
+    \\ strip_tac \\ gs [])
+  \\ Cases_on ‘op = Aupdate_unsafe’ \\ gs []
+  >- (
+    rw [do_app_cases] \\ gs [v_ok_def]
+    \\ gvs [store_lookup_def, store_assign_def, EVERY_EL, EL_LUPDATE]
+    \\ rw [] \\ gs [EVERY_EL, EL_LUPDATE, ref_ok_def]
+    \\ first_assum (irule_at Any)
+    \\ rw [] \\ gs []
+    >- (
+      irule kernel_loc_ok_LUPDATE1 \\ gs []
+      \\ strip_tac \\ gvs [v_ok_def])
+    \\ gvs [oEL_LUPDATE, CaseEq "bool", SF SFY_ss]
+    \\ rw [ref_ok_def, EVERY_EL, EL_LUPDATE] \\ rw []
+    \\ first_x_assum drule
+    \\ gs [LLOOKUP_EQ_EL, ref_ok_def, EVERY_EL])
+  \\ Cases_on ‘op = Asub_unsafe’ \\ gs []
+  >- (
+    rw [do_app_cases] \\ gs [SF SFY_ss]
+    \\ gvs [store_lookup_def, v_ok_def, LLOOKUP_EQ_EL, EVERY_EL]
+    \\ first_assum (irule_at Any) \\ gs []
+    \\ first_x_assum drule_all
+    \\ gs [ref_ok_def, EVERY_EL])
+  \\ Cases_on ‘op = Aupdate’ \\ gs []
+  >- (
+    rw [do_app_cases] \\ gs [v_ok_def, SF SFY_ss]
+    \\ gvs [store_lookup_def, store_assign_def, EVERY_EL, EL_LUPDATE]
+    \\ first_assum (irule_at Any) \\ gs [LLOOKUP_EQ_EL]
+    \\ rw [ref_ok_def, EVERY_EL, EL_LUPDATE] \\ rw []
+    >- (
+      irule kernel_loc_ok_LUPDATE1 \\ gs []
+      \\ strip_tac \\ gvs [v_ok_def])
+    \\ first_x_assum drule_all
+    \\ gs [ref_ok_def, EVERY_EL])
+  \\ Cases_on ‘op = Alength’ \\ gs []
+  >- (
+    rw [do_app_cases] \\ gs [SF SFY_ss]
+    \\ first_assum (irule_at Any)
+    \\ simp [v_ok_def])
+  \\ Cases_on ‘op = Asub’ \\ gs []
+  >- (
+    rw [do_app_cases] \\ gs [SF SFY_ss]
+    \\ gvs [store_lookup_def, v_ok_def, EVERY_EL, LLOOKUP_EQ_EL]
+    \\ first_assum (irule_at Any) \\ gs []
+    \\ first_x_assum drule_all
+    \\ gs [ref_ok_def, EVERY_EL])
+  \\ Cases_on ‘op = AallocEmpty’ \\ gs []
+  >- (
+    rw [do_app_cases] \\ gs [SF SFY_ss]
+    \\ gvs [v_ok_def, store_alloc_def, EVERY_EL, LLOOKUP_EQ_EL]
+    \\ first_assum (irule_at Any) \\ gs []
+    \\ rw [EL_APPEND_EQN] \\ gs [NOT_LESS, LESS_OR_EQ, ref_ok_def]
+    >- (
+      gs [kernel_loc_ok_def, LLOOKUP_EQ_EL, EL_APPEND_EQN]
+      \\ first_x_assum (drule_then strip_assume_tac)
+      \\ rw [] \\ gs [SF SFY_ss])
+    \\ strip_tac
+    \\ first_x_assum (drule_then assume_tac)
+    \\ drule kernel_loc_ok_LENGTH \\ gs [])
+  \\ Cases_on ‘op = Aalloc’ \\ gs []
+  >- (
+    rw [do_app_cases] \\ gs [SF SFY_ss]
+    \\ gvs [v_ok_def, store_alloc_def, EVERY_EL, LLOOKUP_EQ_EL]
+    \\ first_assum (irule_at Any) \\ gs []
+    \\ rw [EL_APPEND_EQN] \\ gs [NOT_LESS, LESS_OR_EQ, ref_ok_def]
+    >- (
+      gs [kernel_loc_ok_def, LLOOKUP_EQ_EL, EL_APPEND_EQN]
+      \\ first_x_assum (drule_then strip_assume_tac)
+      \\ rw [] \\ gs [SF SFY_ss])
+    \\ strip_tac
+    \\ first_x_assum (drule_then assume_tac)
+    \\ drule kernel_loc_ok_LENGTH \\ gs [])
+  \\ Cases_on ‘op = Vlength’ \\ gs []
+  >- (
+    rw [do_app_cases] \\ gs [SF SFY_ss]
+    \\ first_assum (irule_at Any)
+    \\ simp [v_ok_def])
+  \\ Cases_on ‘op = Vsub’ \\ gs []
+  >- (
+    rw [do_app_cases] \\ gs [SF SFY_ss]
+    \\ first_assum (irule_at Any)
+    \\ gs [v_ok_def, EVERY_EL])
+  \\ Cases_on ‘op = VfromList’ \\ gs []
+  >- (
+    rw [do_app_cases] \\ gs [SF SFY_ss]
+    \\ first_assum (irule_at Any)
+    \\ drule_all v_ok_v_to_list
+    \\ simp [v_ok_def])
+  \\ Cases_on ‘op = Strcat’ \\ gs []
+  >- (
+    rw [do_app_cases] \\ gs [SF SFY_ss]
+    \\ first_assum (irule_at Any)
+    \\ simp [v_ok_def])
+  \\ Cases_on ‘op = Strlen’ \\ gs []
+  >- (
+    rw [do_app_cases] \\ gs [SF SFY_ss]
+    \\ first_assum (irule_at Any)
+    \\ simp [v_ok_def])
+  \\ Cases_on ‘op = Strsub’ \\ gs []
+  >- (
+    rw [do_app_cases] \\ gs [SF SFY_ss]
+    \\ first_assum (irule_at Any)
+    \\ simp [v_ok_def])
+  \\ Cases_on ‘op = Explode’ \\ gs []
+  >- (
+    rw [do_app_cases] \\ gs [SF SFY_ss]
+    \\ first_assum (irule_at Any)
+    \\ rename1 ‘MAP _ xs’
+    \\ qid_spec_tac ‘xs’
+    \\ Induct \\ simp [list_to_v_def, v_ok_def])
+  \\ Cases_on ‘op = Implode’ \\ gs []
+  >- (
+    rw [do_app_cases] \\ gs [SF SFY_ss]
+    \\ first_assum (irule_at Any)
+    \\ simp [v_ok_def])
+  \\ Cases_on ‘∃opb. op = Chopb opb’ \\ gs []
+  >- (
+    rw [do_app_cases] \\ gs [SF SFY_ss]
+    \\ first_assum (irule_at Any)
+    \\ simp [Boolv_def]
+    \\ rw [v_ok_def])
+  \\ Cases_on ‘op = Chr’ \\ gs []
+  >- (
+    rw [do_app_cases] \\ gs [SF SFY_ss]
+    \\ first_assum (irule_at Any)
+    \\ simp [v_ok_def])
+  \\ Cases_on ‘op = Ord’ \\ gs []
+  >- (
+    rw [do_app_cases] \\ gs [SF SFY_ss]
+    \\ first_assum (irule_at Any)
+    \\ simp [v_ok_def])
+  \\ Cases_on ‘op = CopyAw8Aw8’ \\ gs []
+  >- (
+    rw [do_app_cases] \\ gs [v_ok_def, SF SFY_ss]
+    \\ first_assum (irule_at Any) \\ gs [LLOOKUP_EQ_EL]
+    \\ gvs [store_assign_def, EL_LUPDATE, EVERY_EL]
+    \\ rw [ref_ok_def]
+    \\ irule kernel_loc_ok_LUPDATE1
+    \\ rpt strip_tac \\ gvs [])
+  \\ Cases_on ‘op = CopyAw8Str’ \\ gs []
+  >- (
+    rw [do_app_cases] \\ gs [v_ok_def, SF SFY_ss]
+    \\ first_assum (irule_at Any)
+    \\ gvs [store_assign_def, EL_LUPDATE, EVERY_EL, LLOOKUP_EQ_EL]
+    \\ rw [ref_ok_def]
+    \\ irule kernel_loc_ok_LUPDATE1
+    \\ rpt strip_tac \\ gvs [])
+  \\ Cases_on ‘op = CopyStrAw8’ \\ gs []
+  >- (
+    rw [do_app_cases] \\ gs [v_ok_def, SF SFY_ss]
+    \\ first_assum (irule_at Any)
+    \\ gvs [store_assign_def, EL_LUPDATE, EVERY_EL, LLOOKUP_EQ_EL]
+    \\ rw [ref_ok_def]
+    \\ irule kernel_loc_ok_LUPDATE1
+    \\ rpt strip_tac \\ gvs [])
+  \\ Cases_on ‘op = CopyStrStr’ \\ gs []
+  >- (
+    rw [do_app_cases] \\ gs [SF SFY_ss]
+    \\ first_assum (irule_at Any)
+    \\ simp [v_ok_def])
+  \\ Cases_on ‘∃n. op = WordToInt n’ \\ gs []
+  >- (
+    rw [do_app_cases] \\ gs [SF SFY_ss]
+    \\ first_assum (irule_at Any)
+    \\ simp [v_ok_def])
+  \\ Cases_on ‘∃n. op = WordFromInt n’ \\ gs []
+  >- (
+    rw [do_app_cases] \\ gs [SF SFY_ss]
+    \\ first_assum (irule_at Any)
+    \\ simp [v_ok_def])
+  \\ Cases_on ‘op = Aw8update’ \\ gs []
+  >- (
+    rw [do_app_cases] \\ gs [v_ok_def, SF SFY_ss]
+    \\ first_assum (irule_at Any)
+    \\ gvs [store_assign_def, EL_LUPDATE, EVERY_EL, LLOOKUP_EQ_EL]
+    \\ rw [ref_ok_def]
+    \\ irule kernel_loc_ok_LUPDATE1
+    \\ rpt strip_tac \\ gvs [])
+  \\ Cases_on ‘op = Aw8sub’ \\ gs []
+  >- (
+    rw [do_app_cases] \\ gs [SF SFY_ss]
+    \\ first_assum (irule_at Any)
+    \\ simp [v_ok_def])
+  \\ Cases_on ‘op = Aw8length’ \\ gs []
+  >- (
+    rw [do_app_cases] \\ gs [SF SFY_ss]
+    \\ first_assum (irule_at Any)
+    \\ simp [v_ok_def])
+  \\ Cases_on ‘op = Aw8alloc’ \\ gs []
+  >- (
+    rw [do_app_cases] \\ gs [SF SFY_ss]
+    \\ gvs [v_ok_def, store_alloc_def, EVERY_EL, LLOOKUP_EQ_EL]
+    \\ first_assum (irule_at Any) \\ gs []
+    \\ rw [EL_APPEND_EQN] \\ gs [NOT_LESS, LESS_OR_EQ, ref_ok_def]
+    >- (
+      gs [kernel_loc_ok_def, LLOOKUP_EQ_EL, EL_APPEND_EQN]
+      \\ first_x_assum (drule_then strip_assume_tac)
+      \\ rw [] \\ gs [SF SFY_ss])
+    \\ strip_tac
+    \\ first_x_assum (drule_then assume_tac)
+    \\ drule kernel_loc_ok_LENGTH \\ gs [])
+  \\ Cases_on ‘∃top. op = FP_top top’ \\ gs []
+  >- (
+    rw [do_app_cases] \\ gs [SF SFY_ss]
+    \\ first_assum (irule_at Any)
+    \\ simp [v_ok_def])
+  \\ Cases_on ‘∃bop. op = FP_bop bop’ \\ gs []
+  >- (
+    rw [do_app_cases] \\ gs [SF SFY_ss]
+    \\ first_assum (irule_at Any)
+    \\ simp [v_ok_def])
+  \\ Cases_on ‘∃uop. op = FP_uop uop’ \\ gs []
+  >- (
+    rw [do_app_cases] \\ gs [SF SFY_ss]
+    \\ first_assum (irule_at Any)
+    \\ simp [v_ok_def])
+  \\ Cases_on ‘∃cmp. op = FP_cmp cmp’ \\ gs []
+  >- (
+    rw [do_app_cases] \\ gs [SF SFY_ss]
+    \\ first_assum (irule_at Any)
+    \\ simp [Boolv_def]
+    \\ rw [v_ok_def])
+  \\ Cases_on ‘∃opn. op = Opn opn’ \\ gs []
+  >- (
+    rw [do_app_cases] \\ gs [SF SFY_ss]
+    \\ first_assum (irule_at Any)
+    \\ simp [v_ok_def])
+  \\ Cases_on ‘∃opb. op = Opb opb’ \\ gs []
+  >- (
+    rw [do_app_cases] \\ gs [SF SFY_ss]
+    \\ first_assum (irule_at Any)
+    \\ simp [Boolv_def]
+    \\ rw [v_ok_def])
+  \\ Cases_on ‘∃sz opw. op = Opw sz opw’ \\ gs []
+  >- (
+    rw [do_app_cases] \\ gs [SF SFY_ss]
+    \\ first_assum (irule_at Any)
+    \\ simp [v_ok_def])
+  \\ Cases_on ‘∃sz sh n. op = Shift sz sh n’ \\ gs []
+  >- (
+    rw [do_app_cases] \\ gs [SF SFY_ss]
+    \\ first_assum (irule_at Any)
+    \\ simp [v_ok_def])
+  \\ Cases_on ‘op = Equality’ \\ gs []
+  >- (
+    rw [do_app_cases] \\ gs [SF SFY_ss]
+    \\ first_assum (irule_at Any)
+    \\ simp [Boolv_def]
+    \\ rw [v_ok_def])
+  \\ Cases_on ‘op = Opderef’ \\ gs []
+  >- (
+    rw [do_app_cases] \\ gs [SF SFY_ss]
+    \\ first_assum (irule_at Any)
+    \\ gs [v_ok_def, store_lookup_def, EVERY_EL, LLOOKUP_EQ_EL]
+    \\ first_x_assum drule \\ gs [ref_ok_def])
+  \\ Cases_on ‘op = Opassign’ \\ gs []
+  >- (
+    rw [do_app_cases] \\ gs [SF SFY_ss]
+    \\ first_assum (irule_at Any)
+    \\ gvs [v_ok_def, store_assign_def, EVERY_EL, EL_LUPDATE, LLOOKUP_EQ_EL]
+    \\ rw [ref_ok_def]
+    \\ irule kernel_loc_ok_LUPDATE1
+    \\ rpt strip_tac \\ gs [])
+  \\ Cases_on ‘op = Opref’ \\ gs []
+  >- (
+    rw [do_app_cases] \\ gs [SF SFY_ss]
+    \\ first_assum (irule_at Any)
+    \\ gvs [v_ok_def, store_alloc_def, ref_ok_def, LLOOKUP_EQ_EL]
+    \\ rw [DISJ_EQ_IMP] \\ rpt strip_tac
+    >- (
+      gs [kernel_loc_ok_def, LLOOKUP_EQ_EL, EL_APPEND_EQN]
+      \\ first_x_assum (drule_then strip_assume_tac)
+      \\ rw [] \\ gs [SF SFY_ss])
+    \\ rw [EL_APPEND_EQN] \\ gs [NOT_LESS, LESS_OR_EQ, ref_ok_def]
+    \\ first_x_assum (drule_then assume_tac)
+    \\ drule kernel_loc_ok_LENGTH \\ gs [])
+  \\ Cases_on ‘op’ \\ gs [] *)
+QED
+
+(* TODO Move up *)
+Theorem res_rel_list_result:
+  res_rel R1 R2 x y ⇒
+    res_rel (LIST_REL R1) R2 (list_result x) (list_result y)
+Proof
+  Cases_on ‘x’ \\ Cases_on ‘y’ \\ gs [list_result_def]
+  \\ rename1 ‘_ _ (Rerr e1) (Rerr e2)’
+  \\ Cases_on ‘e1’ \\ Cases_on ‘e2’ \\ gs []
+QED
+
+(* TODO Move up *)
+Theorem res_rel_mono:
+  res_rel R1 R2 x y ∧
+  (∀x y. R1 x y ⇒ Q1 x y) ∧
+  (∀x y. R2 x y ⇒ Q2 x y) ⇒
+    res_rel Q1 Q2 x y
+Proof
+  rw []
+  \\ Cases_on ‘x’ \\ Cases_on ‘y’ \\ gs []
+  \\ rename1 ‘_ _ (Rerr e1) (Rerr e2)’
+  \\ Cases_on ‘e1’ \\ Cases_on ‘e2’ \\ gs []
+QED
+
+Theorem evaluate_update_Op:
+  op ≠ Opapp ∧ op ≠ Eval ⇒ ^(get_goal "App")
+Proof
+  rw [evaluate_def]
+  \\ gvs [CaseEqs ["prod", "result", "option"], PULL_EXISTS]
+  \\ first_x_assum (drule_all_then strip_assume_tac)
+  \\ Cases_on ‘res1’ \\ gs []
+  \\ first_assum (irule_at Any) \\ gs []
+  \\ dxrule_then assume_tac EVERY2_REVERSE
+  \\ drule_all_then strip_assume_tac do_app_update
+  \\ gs [OPTREL_def]
+  \\ rpt (pairarg_tac \\ gvs [])
+  \\ first_assum (irule_at Any)
+  \\ first_assum (irule_at Any)
+  \\ irule_at Any res_rel_list_result
+  \\ rename1 ‘res_rel _ _ r1 r2’
+  \\ Cases_on ‘r1’ \\ Cases_on ‘r2’ \\ gs []
+  >~ [‘res_rel _ _ (Rerr e1) (Rerr e2)’] >- (
+    Cases_on ‘e1’ \\ Cases_on ‘e2’ \\ gs []
+    \\ cheat (* mono *))
+  \\ cheat (* same *)
+QED
+
+Theorem evaluate_update_Opapp:
+  op = Opapp ⇒ ^(get_goal "App")
+Proof
+  rw [evaluate_def]
+  \\ gvs [CaseEqs ["option", "prod", "result", "bool"], PULL_EXISTS]
+  >~ [‘do_opapp _ = NONE’] >- (
+    first_x_assum (drule_all_then strip_assume_tac)
+    \\ first_assum (irule_at Any) \\ gs []
+    \\ first_assum (irule_at Any) \\ gs []
+    \\ Cases_on ‘res1’ \\ gs []
+    \\ cheat)
+  >~ [‘s.clock = 0’] >- (
+    first_x_assum (drule_all_then strip_assume_tac)
+    \\ first_assum (irule_at Any) \\ gs []
+    \\ first_assum (irule_at Any) \\ gs []
+    \\ Cases_on ‘res1’ \\ gs []
+    \\ cheat)
+  \\ first_x_assum (drule_all_then strip_assume_tac) \\ gs []
+  \\ Cases_on ‘res1’ \\ gs []
+  \\ cheat
+QED
+
+Theorem evaluate_update_App:
+  ^(get_goal "App")
+Proof
+  Cases_on ‘op = Opapp’ >- (match_mp_tac evaluate_update_Opapp \\ gs [])
+  \\ Cases_on ‘op = Eval’ >- (match_mp_tac evaluate_update_Eval \\ gs [])
+  \\ match_mp_tac evaluate_update_Op \\ gs []
+QED
+
+Theorem v_rel_Boolv:
+  state_rel l fr ft fe s t ∧
+  v_rel fr ft fe v1 v2 ⇒
+    ∀b. v1 = Boolv b ⇔ v2 = Boolv b
+Proof
+  rw [Boolv_def, state_rel_def] \\ rw [EQ_IMP_THM]
+  \\ gvs [v_rel_def, OPTREL_def, Once stamp_rel_cases, flookup_thm]
+  \\ qpat_x_assum ‘INJ ($' ft) _ _’ mp_tac \\ rw [INJ_DEF]
+QED
+
+Theorem v_rel_do_log:
+  state_rel l fr ft fe s t ∧
+  v_rel fr ft fe v1 v2 ∧
+  do_log lop v1 x = res ⇒
+    case res of
+      SOME (Val v) =>
+        ∃w. do_log lop v2 x = SOME (Val w) ∧
+            v_rel fr ft fe v w
+    | _ => do_log lop v2 x = res
+Proof
+  rw [] \\ gs []
+  \\ drule_all_then assume_tac v_rel_Boolv \\ gs []
+  \\ gs [do_log_def]
+  \\ rw [] \\ gs []
+QED
+
+Theorem evaluate_update_Log:
+  ^(get_goal "Log")
+Proof
+  rw [evaluate_def]
+  \\ gvs [CaseEqs ["option", "prod", "result", "bool", "exp_or_val"],
+          PULL_EXISTS]
+  \\ first_x_assum (drule_all_then strip_assume_tac) \\ gs []
+  \\ Cases_on ‘res1’ \\ gs []
+  >~ [‘res_rel _ _ (Rerr err1) (Rerr err2)’] >- (
+    Cases_on ‘err1’ \\ Cases_on ‘err2’ \\ gs []
+    \\ gs [SF SFY_ss])
+  \\ drule_then strip_assume_tac evaluate_sing \\ gvs []
+  \\ drule_all_then assume_tac v_rel_do_log \\ gs [SF SFY_ss]
+  \\ drule_all_then assume_tac env_rel_update
+  \\ first_x_assum (drule_all_then strip_assume_tac) \\ gs []
+  \\ first_assum (irule_at Any) \\ gs []
+  \\ irule_at Any SUBMAP_TRANS \\ first_assum (irule_at Any) \\ gs []
+  \\ irule_at Any SUBMAP_TRANS \\ first_assum (irule_at Any) \\ gs []
+  \\ irule_at Any SUBMAP_TRANS \\ first_assum (irule_at Any) \\ gs []
+QED
+
+Theorem evaluate_update_If:
+  ^(get_goal "If")
+Proof
+  rw [evaluate_def]
+  \\ gvs [CaseEqs ["option", "prod", "result", "bool", "exp_or_val"],
+          PULL_EXISTS]
+  \\ first_x_assum (drule_all_then strip_assume_tac) \\ gs []
+  \\ Cases_on ‘res1’ \\ gs []
+  >~ [‘res_rel _ _ (Rerr err1) (Rerr err2)’] >- (
+    Cases_on ‘err1’ \\ Cases_on ‘err2’ \\ gs []
+    \\ gs [SF SFY_ss])
+  \\ drule_then strip_assume_tac evaluate_sing \\ gvs []
+  \\ drule_all_then assume_tac v_rel_Boolv
+  \\ gvs [do_if_def, CaseEqs ["option", "bool"], SF SFY_ss]
+  \\ drule_all_then assume_tac env_rel_update
+  \\ first_x_assum (drule_all_then strip_assume_tac) \\ gs []
+  \\ first_assum (irule_at Any) \\ gs []
+  \\ irule_at Any SUBMAP_TRANS \\ first_assum (irule_at Any) \\ gs []
+  \\ irule_at Any SUBMAP_TRANS \\ first_assum (irule_at Any) \\ gs []
+  \\ irule_at Any SUBMAP_TRANS \\ first_assum (irule_at Any) \\ gs []
+QED
+
+Theorem evaluate_update_Mat:
+  ^(get_goal "Mat")
+Proof
+  rw [evaluate_def]
+  \\ gvs [CaseEqs ["option", "prod", "result", "bool"], PULL_EXISTS]
+  \\ first_x_assum (drule_all_then strip_assume_tac) \\ gs []
+  \\ Cases_on ‘res1’ \\ gs []
+  >~ [‘res_rel _ _ (Rerr err1) (Rerr err2)’] >- (
+    Cases_on ‘err1’ \\ Cases_on ‘err2’ \\ gs []
+    \\ gs [SF SFY_ss])
+  \\ drule_then strip_assume_tac evaluate_sing \\ gvs []
+  \\ drule_all_then assume_tac env_rel_update
+  \\ ‘v_rel fr1 ft1 fe1 bind_exn_v bind_exn_v’
+    by (rw [bind_exn_v_def, v_rel_def, Once stamp_rel_cases]
+        \\ gs [state_rel_def, bind_stamp_def, SF SFY_ss])
+  >- (
+    first_x_assum (drule_all_then strip_assume_tac) \\ gs []
+    \\ first_assum (irule_at Any)
+    \\ first_assum (irule_at Any) \\ gs []
+    \\ cheat (* can_pmatch_all *)
+  )
+  \\ cheat (* can_pmatch_all *)
+QED
+
+Theorem evaluate_update_Let:
+  ^(get_goal "Let")
+Proof
+  rw [evaluate_def]
+  \\ gvs [CaseEqs ["option", "prod", "result", "bool"], PULL_EXISTS]
+  \\ first_x_assum (drule_all_then strip_assume_tac) \\ gs []
+  \\ Cases_on ‘res1’ \\ gs []
+  >~ [‘res_rel _ _ (Rerr err1) (Rerr err2)’] >- (
+    Cases_on ‘err1’ \\ Cases_on ‘err2’ \\ gs []
+    \\ gs [SF SFY_ss])
+  \\ drule_then strip_assume_tac evaluate_sing \\ gvs []
+  \\ drule_all_then assume_tac env_rel_update
+  \\ rename1 ‘v_rel fr1 ft1 fe1 v1 v2’
+  \\ ‘env_rel fr1 ft1 fe1 (env with v := nsOptBind xo v1 env.v)
+                          (env1 with v := nsOptBind xo v2 env1.v)’
+    by (Cases_on ‘xo’ \\ gs [namespaceTheory.nsOptBind_def, env_rel_def]
+        \\ conj_tac \\ Cases \\ gs [namespacePropsTheory.nsLookup_nsBind]
+        \\ rename1 ‘Short m’
+        \\ Cases_on ‘x = m’
+        \\ gs [namespacePropsTheory.nsLookup_nsBind])
+  \\ first_x_assum (drule_all_then strip_assume_tac) \\ gs []
+  \\ first_assum (irule_at Any) \\ gs []
+  \\ irule_at Any SUBMAP_TRANS \\ first_assum (irule_at Any) \\ gs []
+  \\ irule_at Any SUBMAP_TRANS \\ first_assum (irule_at Any) \\ gs []
+  \\ irule_at Any SUBMAP_TRANS \\ first_assum (irule_at Any) \\ gs []
+QED
+
+Theorem NOT_NIL_CONS:
+  xs ≠ [] ⇔ ∃y ys. xs = y::ys
+Proof
+  Cases_on ‘xs’ \\ gs []
+QED
+
+Theorem evaluate_update_Letrec:
+  ^(get_goal "Letrec")
+Proof
+  rw [evaluate_def]
+  >~ [‘¬ALL_DISTINCT _’] >- (
+    first_assum (irule_at Any) \\ gs [])
+  \\ ‘env_rel fr ft fe (env with v := build_rec_env funs env env.v)
+                       (env1 with v := build_rec_env funs env1 env1.v)’
+    suffices_by (
+      strip_tac
+      \\ first_x_assum (drule_all_then strip_assume_tac)
+      \\ first_assum (irule_at Any) \\ gs [])
+  \\ gs [env_rel_def]
+  \\ simp [semanticPrimitivesPropsTheory.build_rec_env_merge,
+           namespacePropsTheory.nsLookup_nsAppend_some,
+           namespacePropsTheory.nsLookup_nsAppend_none,
+           namespacePropsTheory.nsLookup_alist_to_ns_some,
+           namespacePropsTheory.nsLookup_alist_to_ns_none]
+  \\ rw [] \\ gs [SF SFY_ss]
+  \\ gs [ALOOKUP_NONE, MEM_MAP, FORALL_PROD]
+  \\ rw [DISJ_EQ_IMP] \\ gs [NOT_NIL_CONS, PULL_EXISTS]
+  >- (
+    drule_then assume_tac ALOOKUP_MEM
+    \\ gvs [MEM_MAP, EXISTS_PROD, v_rel_def, PULL_EXISTS, DISJ_EQ_IMP]
+    \\ rename1 ‘MEM (x1,x2,x3) funs’
+    \\ Cases_on ‘ALOOKUP (MAP (λ(f,n,e). (f,Recclosure env1 funs f)) funs) x1’
+    \\ gs [ALOOKUP_NONE, MEM_MAP]
+    \\ ‘FST = (λ(x:varN,y:varN,z:exp). x)’
+      by rw [FUN_EQ_THM, ELIM_UNCURRY]
+    \\ ‘ALL_DISTINCT (MAP FST funs)’
+      by gs []
+    \\ drule_then assume_tac MEM_ALOOKUP \\ gvs [FORALL_PROD]
+    \\ drule_then assume_tac ALOOKUP_MEM \\ gs [MEM_MAP, EXISTS_PROD])
+  \\ first_x_assum (drule_all_then strip_assume_tac)
+  \\ first_assum (irule_at Any) \\ gs []
+QED
+
+Theorem evaluate_update_Tannot:
+  ^(get_goal "Tannot")
+Proof
+  rw [evaluate_def]
+QED
+
+Theorem evaluate_update_Lannot:
+  ^(get_goal "Lannot")
+Proof
+  rw [evaluate_def]
+QED
+
+Theorem evaluate_update_pmatch_Nil:
+  ^(get_goal "[]:(pat # exp) list")
+Proof
+  rw [evaluate_def] \\ gs []
+  \\ first_assum (irule_at Any) \\ gs []
+QED
+
+Theorem evaluate_update_pmatch_Cons:
+  ^(get_goal "_::_:(pat # exp) list")
+Proof
+  rw [evaluate_def]
+  \\ gs [CaseEqs ["match_result"]]
+  \\ cheat
+QED
+
+Theorem evaluate_update_decs_Nil:
+  ^(get_goal "[]:dec list")
+Proof
+  rw [evaluate_decs_def, extend_dec_env_def]
+  \\ first_assum (irule_at Any) \\ gs [SF SFY_ss]
+QED
+
+Theorem evaluate_update_decs_Cons:
+  ^(get_goal "_::_::_:dec list")
+Proof
+  rw [evaluate_decs_def]
+  \\ gvs [CaseEqs ["prod", "result"], PULL_EXISTS]
+  \\ first_x_assum (drule_all_then strip_assume_tac) \\ gs []
+  \\ Cases_on ‘res1’ \\ gs []
+  >~ [‘res_rel _ _ (Rerr _) (Rerr _)’] >- (
+    first_assum (irule_at Any) \\ gs []
+    \\ first_assum (irule_at Any) \\ gs [])
+  \\ first_x_assum (drule_all_then strip_assume_tac)
+  \\ first_assum (irule_at (Pat ‘state_rel’))
+  \\ first_assum (irule_at Any)
+  \\ irule_at Any EQ_REFL
+  \\ irule_at Any SUBMAP_TRANS \\ first_assum (irule_at Any) \\ gs []
+  \\ irule_at Any SUBMAP_TRANS \\ first_assum (irule_at Any) \\ gs []
+  \\ irule_at Any SUBMAP_TRANS \\ first_assum (irule_at Any) \\ gs []
+  \\ gs [combine_dec_result_def]
+  \\ rpt CASE_TAC \\ gs []
+  \\ cheat (* env_rel_extend_dec_env *)
+QED
+
+Theorem evaluate_update_decs_Dlet:
+  ^(get_goal "Dlet")
+Proof
+  rw [evaluate_decs_def]
+  >~ [‘¬ALL_DISTINCT _’] >- (
+    first_assum (irule_at Any) \\ gs [SF SFY_ss])
+  \\ gvs [CaseEqs ["prod", "result"], PULL_EXISTS]
+  \\ first_x_assum (drule_all_then strip_assume_tac) \\ gs []
+  \\ Cases_on ‘res1’ \\ gs []
+  >~ [‘res_rel _ _ (Rerr err1) (Rerr err2)’] >- (
+    Cases_on ‘err1’ \\ Cases_on ‘err2’ \\ gs []
+    \\ first_assum (irule_at Any) \\ gs [SF SFY_ss])
+  \\ first_assum (irule_at Any) \\ gs [SF SFY_ss]
+  \\ cheat (* pmatch, extend_dec_env *)
+QED
+
+Theorem evaluate_update_decs_Dletrec:
+  ^(get_goal "Dletrec")
+Proof
+  rw [evaluate_decs_def]
+  >~ [‘¬ALL_DISTINCT _’] >- (
+    first_assum (irule_at Any) \\ gs [])
+  \\ gvs [CaseEqs ["prod", "result"], PULL_EXISTS]
+  \\ first_assum (irule_at Any) \\ gs []
+  \\ gs [extend_dec_env_def, env_rel_def, PULL_EXISTS, SF SFY_ss,
+         semanticPrimitivesPropsTheory.build_rec_env_merge,
+         namespacePropsTheory.nsLookup_nsAppend_some,
+         namespacePropsTheory.nsLookup_nsAppend_none,
+         namespacePropsTheory.nsLookup_alist_to_ns_some,
+         namespacePropsTheory.nsLookup_alist_to_ns_none,
+         NOT_NIL_CONS, ALOOKUP_NONE, MEM_MAP, FORALL_PROD]
+  \\ Cases \\ gs []
+  \\ strip_tac
+  \\ rename1 ‘Short n’
+  \\ ‘OPTREL (v_rel fr ft fe)
+             (ALOOKUP (MAP (λ(f,n,e). (f,Recclosure env funs f)) funs) n)
+             (ALOOKUP (MAP (λ(f,n,e). (f,Recclosure env1 funs f)) funs) n)’
+    by (rw [OPTREL_def]
+        \\ Cases_on ‘ALOOKUP (MAP (λ(f,n,e).(f,Recclosure env funs f)) funs) n’
+        \\ gs [ALOOKUP_NONE, MAP_MAP_o, o_DEF, LAMBDA_PROD]
+        \\ drule_then assume_tac ALOOKUP_MEM
+        \\ gvs [MEM_MAP, EXISTS_PROD]
+        \\ Cases_on ‘ALOOKUP (MAP (λ(f,n,e).(f,Recclosure env1 funs f)) funs) n’
+        \\ gs [ALOOKUP_NONE, MAP_MAP_o, o_DEF, LAMBDA_PROD, MEM_MAP,
+               EXISTS_PROD, v_rel_def]
+        \\ drule_then assume_tac ALOOKUP_MEM
+        \\ gs [MEM_MAP, EXISTS_PROD])
+  \\ gs [OPTREL_def]
+  \\ drule_then assume_tac ALOOKUP_MEM
+  \\ gvs [MEM_MAP, EXISTS_PROD, v_rel_def]
+  \\ dsimp [] \\ rw [v_rel_def]
+QED
+
+Theorem evaluate_update_decs_Dtype:
+  ^(get_goal "Dtype")
+Proof
+  cheat (*
+  rw [evaluate_decs_def]
+  >~ [‘¬EVERY check_dup_ctors _’] >- (
+    gs [state_ok_def]
+    \\ first_assum (irule_at Any) \\ gs [])
+  \\ gvs [CaseEqs ["prod", "semanticPrimitives$result"], state_ok_def]
+  \\ first_assum (irule_at Any) \\ gs []
+  \\ conj_tac
+  >- (
+    rw []
+    \\ first_x_assum drule \\ gs [])
+  \\ gs [extend_dec_env_def, build_tdefs_def, env_ok_def,
+         nsLookup_nsAppend_some, nsLookup_alist_to_ns_some, SF SFY_ss]
+  \\ rw [] \\ gs [SF SFY_ss]
+  \\ ‘∀m tds n l t k.
+        nsLookup (build_tdefs m tds) n = SOME (l, TypeStamp t k) ⇒
+          m ≤ k’
+    by (ho_match_mp_tac build_tdefs_ind
+        \\ simp [build_tdefs_def, nsLookup_nsAppend_some,
+                 nsLookup_alist_to_ns_some, SF SFY_ss]
+        \\ rw [] \\ gs [SF SFY_ss]
+        >- (
+          first_x_assum drule
+          \\ gs [])
+        \\ drule_then assume_tac ALOOKUP_MEM
+        \\ gs [build_constrs_def, MEM_MAP, EXISTS_PROD])
+  \\ first_x_assum (drule_then assume_tac)
+  \\ first_x_assum drule_all \\ gs [] *)
+QED
+
+Theorem evaluate_update_decs_Dtabbrev:
+  ^(get_goal "Dtabbrev")
+Proof
+  rw [evaluate_decs_def]
+  \\ first_assum (irule_at Any)
+  \\ cheat
+QED
+
+Theorem evaluate_update_decs_Denv:
+  ^(get_goal "Denv")
+Proof
+  cheat (*
+  rw [evaluate_decs_def]
+  \\ gvs [CaseEqs ["option", "prod"]]
+  \\ gs [state_ok_def]
+  \\ first_assum (irule_at Any) \\ gs []
+  \\ gs [env_ok_def, extend_dec_env_def, SF SFY_ss]
+  \\ gvs [declare_env_def, CaseEqs ["option", "eval_state", "prod"]]
+  \\ fs [eval_state_ok_def,SF SFY_ss]
+  \\ Cases \\ simp [ml_progTheory.nsLookup_nsBind_compute]
+  \\ rw [] \\ gs [v_ok_def, env_ok_def, nat_to_v_def, SF SFY_ss] *)
+QED
+
+Theorem evaluate_update_decs_Dexn:
+  ^(get_goal "Dexn")
+Proof
+  cheat (*
+  rw [evaluate_decs_def]
+  \\ gvs [CaseEqs ["option", "prod"], state_ok_def]
+  \\ first_assum (irule_at Any) \\ gs []
+  \\ gs [env_ok_def, extend_dec_env_def, SF SFY_ss]
+  \\ Cases \\ simp [ml_progTheory.nsLookup_nsBind_compute]
+  \\ rw [] \\ gs [SF SFY_ss] *)
+QED
+
+Theorem evaluate_update_decs_Dmod:
+  ^(get_goal "Dmod")
+Proof
+  cheat (*
+  rw [evaluate_decs_def]
+  \\ gvs [CaseEqs ["option", "prod", "semanticPrimitives$result"]]
+  \\ first_x_assum (drule_all_then strip_assume_tac)
+  \\ first_assum (irule_at Any) \\ gs []
+  \\ gs [env_ok_def, extend_dec_env_def, SF SFY_ss]
+  \\ conj_tac
+  >- (
+    gs [nsLookup_nsAppend_some, nsLookup_nsLift, nsLookupMod_nsLift]
+    \\ Cases \\ simp []
+    \\ rw [] \\ gs [SF SFY_ss]
+    \\ simp [namespaceTheory.id_to_n_def])
+  \\ Cases \\ gs [ml_progTheory.nsLookup_nsBind_compute, nsLookup_nsAppend_some,
+                  nsLookup_nsLift]
+  \\ rw [] \\ gs [SF SFY_ss] *)
+QED
+
+Theorem evaluate_update_decs_Dlocal:
+  ^(get_goal "Dlocal")
+Proof
+  cheat (*
+  rw [evaluate_decs_def]
+  \\ gvs [CaseEqs ["option", "prod", "semanticPrimitives$result"]]
+  \\ first_x_assum (drule_all_then strip_assume_tac)
+  \\ first_x_assum (drule_all_then strip_assume_tac)
+  \\ CASE_TAC \\ gs []
+  \\ first_assum (irule_at Any) \\ gs []
+  \\ gs [env_ok_def, extend_dec_env_def, SF SFY_ss]
+  \\ conj_tac
+  \\ Cases \\ gs [ml_progTheory.nsLookup_nsBind_compute,
+                nsLookup_nsAppend_some]
+  \\ rw [] \\ gs [SF SFY_ss] *)
+QED
+
+Theorem evaluate_update:
+  ^(evaluate_update ())
+Proof
+  match_mp_tac (the_ind_thm ())
+  \\ rpt conj_tac \\ rpt gen_tac
+  \\ rewrite_tac [evaluate_update_Nil, evaluate_update_Cons,
+                  evaluate_update_Lit, evaluate_update_Raise,
+                  evaluate_update_Handle, evaluate_update_Con,
+                  evaluate_update_Var, evaluate_update_Fun,
+                  evaluate_update_App, evaluate_update_Log,
+                  evaluate_update_If, evaluate_update_Mat,
+                  evaluate_update_Let, evaluate_update_Letrec,
+                  evaluate_update_Tannot, evaluate_update_Lannot,
+                  evaluate_update_pmatch_Nil, evaluate_update_pmatch_Cons,
+                  evaluate_update_decs_Nil, evaluate_update_decs_Cons,
+                  evaluate_update_decs_Dlet, evaluate_update_decs_Dletrec,
+                  evaluate_update_decs_Dtype,
+                  evaluate_update_decs_Dtabbrev,
+                  evaluate_update_decs_Denv, evaluate_update_decs_Dexn,
+                  evaluate_update_decs_Dmod, evaluate_update_decs_Dlocal]
+QED
+
+(* --------------------------------------------------------------------------
+ *
+ * -------------------------------------------------------------------------- *)
+
 Theorem evaluate_decs_skip:
   ∀s env decs t s1 res fr ft fe env1 l.
     evaluate_decs s env decs = (s1,res) ∧
@@ -231,62 +1324,10 @@ Theorem evaluate_decs_skip:
                                                 (extend_dec_env env1' env1))
         (v_rel fr1 ft1 fe1) res res1
 Proof
-  ho_match_mp_tac evaluate_decs_ind \\ rw []
-  >- ((* nil *)
-    simp [extend_dec_env_def]
-    \\ first_assum (irule_at Any) \\ gs [])
-  >- ((* cons *)
-    gvs [evaluate_decs_def, CaseEqs ["prod", "result"], PULL_EXISTS]
-    >~ [‘Rerr err’] >- (
-        first_x_assum (drule_all_then strip_assume_tac) \\ gs []
-        \\ first_assum (irule_at Any)
-        \\ Cases_on ‘res1’ \\ gs [res_rel_def])
-    \\ first_x_assum (drule_all_then strip_assume_tac) \\ gs []
-    \\ Cases_on ‘res1’ \\ gs [res_rel_def]
-    \\ first_x_assum (drule_all_then strip_assume_tac) \\ gs []
-    \\ gs [combine_dec_result_def]
-    \\ cheat)
-  >~ [‘Dlet locs p e’] >- (
-    gvs [evaluate_decs_def, CaseEqs ["prod", "result", "bool", "match_result"],
-         PULL_EXISTS]
-    \\ cheat (* evaluate theorem *))
-  >~ [‘Dletrec locs funs’] >- (
-    cheat
-  )
-  >~ [‘Dtype locs tds’] >- (
-    cheat
-  )
-  >~ [‘Dtabbrev locs tvs tn t’] >- (
-    cheat
-  )
-  >~ [‘Denv n’] >- (
-    cheat
-  )
-  >~ [‘Dexn locs cn ts’] >- (
-    gvs [evaluate_decs_def, CaseEqs ["prod", "result"], PULL_EXISTS]
-    \\ irule_at Any SUBMAP_REFL
-    \\ irule_at Any SUBMAP_REFL
-    \\ drule_then (qspec_then ‘1’ strip_assume_tac)
-                  state_rel_with_next_exn_stamp
-    \\ first_assum (irule_at Any) \\ gs []
-    \\ cheat (* env_rel_extend_dec_env *)
-  )
-  >~ [‘Dmod mn decs’] >- (
-    gvs [evaluate_decs_def, CaseEqs ["prod", "result"], PULL_EXISTS]
-    \\ first_x_assum (drule_all_then strip_assume_tac)
-    \\ first_assum (irule_at Any) \\ gs []
-    \\ Cases_on ‘res1’ \\ gs [res_rel_def, extend_dec_env_def]
-    \\ cheat (* env_rel nsAppend *)
-  )
-  >~ [‘Dlocal ds1 ds2’] >- (
-    gvs [evaluate_decs_def, CaseEqs ["prod", "result"], PULL_EXISTS]
-    \\ first_x_assum (drule_all_then strip_assume_tac)
-    \\ first_assum (irule_at Any) \\ gs []
-    \\ Cases_on ‘res1’ \\ gs [res_rel_def]
-    \\ first_x_assum (drule_all_then strip_assume_tac)
-    \\ first_assum (irule_at Any) \\ gs []
-    \\ cheat (* env_rel transitive *)
-  )
+  rw []
+  \\ drule_all_then strip_assume_tac (el 3 (CONJUNCTS evaluate_update))
+  \\ first_assum (irule_at (Pos last))
+  \\ first_assum (irule_at Any) \\ gs []
 QED
 
 Theorem evaluate_decs_init:
@@ -298,7 +1339,41 @@ Theorem evaluate_decs_init:
      state_rel (LENGTH s.refs) fr ft fe s s ∧
      env_rel fr ft fe (extend_dec_env env init_env) (extend_dec_env env init_env)
 Proof
-  cheat
+  qabbrev_tac ‘s0 = (init_state ffi with clock := ck)’
+  \\ qabbrev_tac ‘l = LENGTH s0.refs’
+  \\ qabbrev_tac ‘fr = FUN_FMAP I (count (LENGTH s0.refs))’
+  \\ qabbrev_tac ‘ft = FUN_FMAP I (count s0.next_type_stamp)’
+  \\ qabbrev_tac ‘fe = FUN_FMAP I (count s0.next_exn_stamp)’
+  \\ ‘state_rel l fr ft fe s0 s0’
+    by (unabbrev_all_tac
+        \\ simp [state_rel_def, ml_progTheory.init_state_def, FLOOKUP_FUN_FMAP,
+                 INJ_DEF, FUN_FMAP_DEF, bool_type_num_def, list_type_num_def])
+  \\ ‘env_rel fr ft fe init_env init_env’
+    by (gs [env_rel_def, ctor_rel_def, ml_progTheory.init_env_def, OPTREL_def]
+        \\ conj_tac \\ Cases \\ simp [namespaceTheory.nsLookup_def]
+        \\ rw [] \\ gs [Once stamp_rel_cases, state_rel_def, bool_type_num_def,
+                        list_type_num_def])
+  \\ strip_tac
+  \\ drule_all_then strip_assume_tac evaluate_decs_skip
+  \\ unabbrev_all_tac \\ gs []
+  \\ conj_tac
+  >- (
+    gs [state_rel_def, FLOOKUP_FUN_FMAP]
+    \\ simp [Once INJ_DEF, FUN_FMAP_DEF]
+    \\ simp [Once INJ_DEF, FUN_FMAP_DEF]
+    \\ simp [Once INJ_DEF, FUN_FMAP_DEF]
+    \\ gvs [ml_progTheory.init_state_def, bool_type_num_def, list_type_num_def]
+    \\ conj_tac >- cheat
+    \\ conj_tac >- cheat
+    \\ conj_tac >- cheat
+    \\ conj_tac >- cheat
+    \\ conj_tac >- cheat
+    \\ conj_tac >- cheat
+    \\ rpt strip_tac
+    \\ first_x_assum (qspec_then ‘n’ mp_tac)
+    \\ rw [] \\ gs []
+    \\ cheat (* ref_rel_mono *))
+  \\ cheat (* env_rel something *)
 QED
 
 val _ = export_theory();
